Scratch.lean
@@ -1,0 +1,3 @@
+import Mathlib.Data.Set.Basic
+example {α : Type} (a : α) : a ∈ (Set.singleton a : Set α) := by
+  simp [Set.singleton]
